probably not gonna work on soundness anymore

typing.lean
@@ -2,18 +2,19 @@ import .core .partial_fun
 
 def ctx := partial_fun var type
 
-inductive well_typed_under : ctx → term → type → Prop
+inductive has_type_under : ctx → term → type → Prop
 | unit {Γ : ctx} :
-    well_typed_under Γ term.unit type.unit
+    has_type_under Γ term.unit type.unit
 
 | var {Γ : ctx} {x : var} {τ : type} :
-    Γ x = τ → well_typed_under Γ (term.var x) τ
+    Γ x = τ → has_type_under Γ (term.var x) τ
 
 | abs {Γ : ctx} {x : var} {e : term} {τ τ' : type} :
-    well_typed_under (extend Γ x τ) e τ' → well_typed_under Γ (term.abs x e) (type.func τ τ')
+    has_type_under (extend Γ x τ) e τ' → has_type_under Γ (term.abs x e) (type.func τ τ')
 
 | app {Γ : ctx} {e₁ e₂ : term} {τ τ' : type} :
-    well_typed_under Γ e₁ (type.func τ τ') → well_typed_under Γ e₂ τ →
-      well_typed_under Γ (term.app e₁ e₂) τ'
+    has_type_under Γ e₁ (type.func τ τ') → has_type_under Γ e₂ τ →
+      has_type_under Γ (term.app e₁ e₂) τ'
 
-def well_typed := well_typed_under emptyf
+@[reducible]
+def has_type := has_type_under emptyf
