partial_fun.lean
@@ -9,36 +9,44 @@ def emptyf : partial_fun α β
 instance : has_emptyc (partial_fun α β) :=
 ⟨emptyf⟩
 
-def dom (f : partial_fun α β) : set α :=
-λ x, ∃ τ, f x = some τ
+inductive dom (f : partial_fun α β) : set α
+| intro (a) (b) : f a = some b → dom a
 
 variable [decidable_eq α]
 
 -- Destructive addition to a context
+@[irreducible]
 def extend (f : partial_fun α β) (x : α) (y : β) : partial_fun α β
 | x' := if x' = x then y else f x'
 
 instance : has_insert (α × β) (partial_fun α β) :=
 ⟨λ ⟨a, b⟩ f, extend f a b⟩
 
-lemma extend_eta (f : partial_fun α β) (x : α) (y : β) :
-  extend f x y = λ x', if x' = x then y else f x' := rfl
+variable (f : partial_fun α β)
 
-lemma extend_same (f : partial_fun α β) (x : α) (y : β) : extend f x y x = y :=
+lemma extend_same (x : α) (y : β) : extend f x y x = y :=
 by unfold extend; simp
 
-lemma extend_diff (f : partial_fun α β) {x x' : α} (y : β) :
+lemma extend_diff {x x' : α} (y : β) :
   x' ≠ x → extend f x y x' = f x' :=
 by intro h; unfold extend; simp [h]
 
-/-instance {f : partial_fun α β} {a} : decidable (∃ b, f a = some b) :=
+lemma extend_comm {x₁ x₂ : α} (y₁ y₂ : β) : x₁ ≠ x₂ →
+  extend (extend f x₁ y₁) x₂ y₂ = extend (extend f x₂ y₂) x₁ y₁ :=
 begin
-  cases f a with b,
+  intro h,
+  apply funext,
+  intro x,
   
-  left, intro h,
-  cases h,
-  contradiction,
+  by_cases x = x₁ with h',
+  simp [h', extend_same,
+        extend_diff _ _ h],
+  
+  rw extend_diff _ _ h',
+  by_cases x = x₂ with h'',
+  
+  simp [h'', extend_same],
 
-  right, existsi b, refl
-end-/
-
+  simp [extend_diff _ _ h',
+        extend_diff _ _ h'']
+end
